theories/typing/lib/refcell/ref_code.v
@@ -56,7 +56,7 @@ Section ref_functions.
      See: https://coq.inria.fr/bugs/show_bug.cgi?id=5326 *)
   Lemma ref_clone_type ty :
     typed_val ref_clone
-      (fn (fun '(α, β) => FP' [α; β]%EL [# &shr{α}(ref β ty)]%T (ref β ty)%T)).
+      (fn (fun '(α, β) => FP [α; β]%EL [# &shr{α}(ref β ty)]%T (ref β ty)%T)).
   Proof.
     intros. iApply type_fn; [solve_typing..|]. iIntros "/= !#".
       iIntros ([α β] ret arg). inv_vec arg=>x. simpl_subst.
