theories/typing/lib/rwlock/rwlockreadguard_code.v
@@ -20,7 +20,7 @@ Section rwlockreadguard_functions.
 
   Lemma rwlockreadguard_deref_type ty :
     typed_val rwlockreadguard_deref
-      (fn (fun '(α, β) => FP' [α; β; α ⊑ β]%EL
+      (fn (fun '(α, β) => FP [α; β; α ⊑ β]%EL
                               [# &shr{α}(rwlockreadguard β ty)] (&shr{α}ty))).
   Proof.
     intros. iApply type_fn; [solve_typing..|]. iIntros "/= !#".
